src/Typing.v
@@ -1,5 +1,5 @@
-From Celsius Require Export Language Notations Helpers.
-Require Import List ListSet.
+From Celsius Require Export Language Notations Helpers LibTactics.
+Require Import List ListSet Psatz.
 Open Scope nat_scope.
 Import ListNotations.
 
@@ -24,6 +24,15 @@ Proof.
 Qed.
 Global Hint Resolve s_mode_trans: typ.
 
+Lemma s_mode_cool: forall Ω1 Ω2, cool Ω1 ⊑ cool Ω2 <-> Ω2 <= Ω1.
+Proof.
+  split; intros.
+  - inversion H; subst; try lia.
+  - assert (Ω2+(Ω1 - Ω2) = Ω1) by lia.
+    pose proof (s_mode_union Ω2 (Ω1 - Ω2)).
+    rewrite H0 in H1.
+    assumption.
+Qed.
 
 (* Subtyping *)
 
@@ -103,7 +112,7 @@ Inductive T_Expr : EnvTyping -> Tpe -> Expr -> Tpe -> Prop :=
 | t_selcool:
     forall Γ T e f U D Ω,
       (Γ, T) ⊢ e : (D, cool Ω) ->
-      f <= Ω ->
+      f < Ω ->
       (fieldType D f = Some U) ->
       (Γ, T) ⊢ (fld e f) : U
 
@@ -129,17 +138,16 @@ Inductive T_Expr : EnvTyping -> Tpe -> Expr -> Tpe -> Prop :=
       (Γ, T) ⊢ (asgn e1 f e2 e3) : U
 
 | t_call:
-    forall Γ T e m args paramTs retT body μ0 μ_m C,
+    forall Γ T e m args argsT U e__m μ0 μ__m C,
       (Γ, T) ⊢ e : (C, μ0) ->
-      μ0 ⊑ μ_m ->
-      methodInfo C m = Some (μ_m, paramTs, retT, body) ->
-      (Γ, T) ⊩ args : paramTs ->
-      (Γ, T) ⊢ (mtd e m args) : retT
+      μ0 ⊑ μ__m ->
+      methodInfo C m = Some (μ__m, argsT, U, e__m) ->
+      (Γ, T) ⊩ args : argsT ->
+      (Γ, T) ⊢ (mtd e m args) : U
 
 | t_call_hot:
     forall Γ T e m args argTs paramTs D body μ0 μ_r C,
       (Γ, T) ⊢ e : (C, hot) ->
-      (C, hot) <: (C, μ0) ->
       methodInfo C m = Some (μ0, paramTs, (D, μ_r), body) ->
       (Γ, T) ⊩ args : argTs ->
       P_hots argTs ->
@@ -168,33 +176,139 @@ Inductive T_Fields: EnvTyping -> Tpe -> (list Field) -> Prop :=
     T_Fields Γ (C, cool (S Ω)) fs ->
     T_Fields Γ (C, cool Ω) (f::fs).
 
-(** ** Method typing *)
-Definition T_Method C m :=
-  match m with
-  | method μ argTs retT body => (argTs, (C, μ)) ⊢ body : retT
-  end.
-Definition T_Methods C (methods: Mtd -> option Method) :=
-  forall id m, methods id = Some m -> T_Method C m.
-
 (** ** Class typing *)
-Definition T_Class C cl :=
-  match cl with
-  | class paramTs fields methods => T_Fields paramTs (C, cold) fields /\ T_Methods C methods
+Definition T_Classes := forall C,
+    match (ct C) with
+    | class Args Flds Mtds =>
+        T_Fields Args (C, cold) Flds /\
+          (forall m μ ρ T e, Mtds m = Some (method μ ρ T e) -> (ρ, (C, μ)) ⊢ e : T)
+    end.
+
+(** ** Program typing *)
+Definition T_Prog :=
+  match ct entry with
+  | class nil nil Mtds =>
+    exists e T, Mtds main = Some (method hot nil T e) /\
+             ((nil, (entry, hot)) ⊢ e : T) /\ T_Classes
+  | _ => False
   end.
 
+(** ** Induction principle for typing *)
+(** The induction assumes the classtable is correct ! *)
+Section typing_ind.
+  (* Parameter typable_classes : T_Classes.*)
 
-(* Definition T_Classes (Ct: list Class) (C: ClN) : *)
-(*   match Ct with *)
-(*   | nil => True *)
-(*   | C::Ct' => (T_Class i C) /\ (T_Classes Ct' (S (proj1_sig i))) *)
-(*   end. *)
+  (* Lemma typable_method : forall m C μ ρ T e__m, *)
+  (*     methodInfo C m = Some (μ, ρ, T, e__m) -> *)
+  (*     ((ρ, (C, μ)) ⊢ e__m : T). *)
+  (* Proof. *)
+  (*   intros. *)
+  (*   destruct (ct C) as [Args Flds Mtds] eqn: H__ct. *)
+  (*   unfold methodInfo in *. *)
+  (*   pose proof (typable_classes C); steps. *)
+  (*   lets : H2 matched0; assumption. *)
+  (* Qed. *)
 
-(* (** ** Program typing *) *)
 
-(* Definition T_Prog := *)
-(*   match (ct entry) with *)
-(*   | Some (class nil nil methods) => *)
-(*     exists e T, methods main = Some (method hot nil T e) /\ *)
-(*     ((nil, (entry, hot)) ⊢ e : T) /\ T_Classes Ξ 0 *)
-(*   | _ => False *)
-(*   end. *)
+  Variable P : forall Γ T e U, ((Γ, T) ⊢ e : U) -> Prop.
+  Variable Pl : forall Γ T el Ul, ((Γ, T) ⊩ el : Ul) -> Prop.
+
+  Variable P_sub: forall Γ T e U U' H__U' H__sub,
+      P Γ T e U' H__U' ->
+      P Γ T e U (t_sub Γ T e U U' H__U' H__sub).
+
+  Variable P_var: forall Γ T x U H__lkp,
+      P Γ T (var x) U (t_var Γ T x U H__lkp).
+
+  Variable P_this: forall Γ T,
+      P Γ T this T (t_this Γ T).
+
+  Variable P_selhot: forall Γ T e f C D μ H__D H__field,
+      P Γ T e (D, hot) H__D ->
+      P Γ T (fld e f) (C, hot) (t_selhot Γ T e f C D μ H__D H__field).
+
+  Variable P_selwarm: forall Γ T e f U D H__D H__field,
+      P Γ T e (D, warm) H__D ->
+      P Γ T (fld e f) U (t_selwarm Γ T e f U D H__D H__field).
+
+  Variable P_selcool: forall Γ T e f U D Ω H__D H__f H__field,
+      P Γ T e (D, cool Ω) H__D ->
+      P Γ T (fld e f) U (t_selcool Γ T e f U D Ω H__D H__f H__field).
+
+  Variable P_new: forall Γ T C args Args Flds Mtds H__ct H__args,
+      Pl Γ T args Args H__args ->
+      P Γ T (new C args) (C, warm) (t_new Γ T C args Args Flds Mtds H__ct H__args).
+
+  Variable P_new_hot: forall Γ T C args argsTs Args Flds Mtds H__ct H__args H__hots H__subs,
+      Pl Γ T args argsTs H__args ->
+      P Γ T (new C args) (C, hot) (t_new_hot Γ T C args argsTs Args Flds Mtds H__ct H__args H__hots H__subs).
+
+  Variable P_block: forall Γ T U e1 f e2 e3 C μ H__fld H__e2 H__e3,
+      P Γ T (fld e1 f) (C, μ) H__fld ->
+      P Γ T e2 (C, hot) H__e2 ->
+      P Γ T e3 U H__e3 ->
+      P Γ T (asgn e1 f e2 e3) U (t_block Γ T U e1 f e2 e3 C μ H__fld H__e2 H__e3).
+
+  Variable P_call: forall Γ T e m args argsT U e__m μ0 μ__m C H__e H__sub H__mtd H__args,
+      P Γ T e (C, μ0) H__e ->
+      Pl Γ T args argsT H__args ->
+      (* P argsT (C, μ__m) e__m U (typable_method m C μ__m argsT U e__m H__mtd) ->*)
+      P Γ T (mtd e m args) U (t_call Γ T e m args argsT U e__m μ0 μ__m C H__e H__sub H__mtd H__args).
+
+  Variable P_call_hot: forall Γ T e m args argTs paramTs D body μ0 μ_r C H__e H__mtd H__args H__hots H__subs,
+      P Γ T e (C, hot) H__e ->
+      Pl Γ T args argTs H__args ->
+      P Γ T (mtd e m args) (D, hot) (t_call_hot Γ T e m args argTs paramTs D body μ0 μ_r C H__e H__mtd H__args H__hots H__subs).
+
+  Variable Pl_nil: forall Γ T,
+      Pl Γ T [] [] (t_exprs_nil Γ T).
+
+  Variable Pl_cons: forall Γ T U Ul e el H__el H__e,
+      P Γ T e U H__e ->
+      Pl Γ T el Ul H__el ->
+      Pl Γ T (e::el) (U::Ul) (t_exprs_cons Γ T Ul el U e H__el H__e).
+
+  Fixpoint typing_ind Γ T e U (typing: (Γ, T) ⊢ e : U) : P Γ T e U typing :=
+    match typing with
+    | t_sub Γ T e U U' H__U' H__sub => P_sub Γ T e U U' H__U' H__sub (typing_ind Γ T e U' H__U')
+    | t_var Γ T x U H__lkp => P_var Γ T x U H__lkp
+    | t_this Γ T => P_this Γ T
+    | t_selhot Γ T e f C D μ H__D H__field =>
+        P_selhot Γ T e f C D μ H__D H__field
+                 (typing_ind Γ T e (D, hot) H__D)
+    | t_selwarm Γ T e f U D H__D H__field =>
+        P_selwarm Γ T e f U D H__D H__field
+                  (typing_ind Γ T e (D, warm) H__D)
+    | t_selcool Γ T e f U D Ω H__D H__f H__field =>
+        P_selcool Γ T e f U D Ω H__D H__f H__field
+                  (typing_ind Γ T e (D, cool Ω) H__D)
+    | t_new Γ T C args Args Flds Mtds H__ct H__args =>
+        P_new Γ T C args Args Flds Mtds H__ct H__args
+              (typing_list_ind Γ T args Args H__args)
+    | t_new_hot Γ T C args argsTs Args Flds Mtds H__ct H__args H__hots H__subs =>
+        P_new_hot Γ T C args argsTs Args Flds Mtds H__ct H__args H__hots H__subs
+                  (typing_list_ind Γ T args argsTs H__args)
+    | t_block Γ T U e1 f e2 e3 C μ H__fld H__e2 H__e3 =>
+        P_block Γ T U e1 f e2 e3 C μ H__fld H__e2 H__e3
+                (typing_ind Γ T (fld e1 f) (C, μ) H__fld)
+                (typing_ind Γ T e2 (C, hot) H__e2)
+                (typing_ind Γ T e3 U H__e3)
+    | t_call Γ T e m args argsT U e__m μ0 μ__m C H__e H__sub H__mtd H__args =>
+        P_call Γ T e m args argsT U e__m μ0 μ__m C H__e H__sub H__mtd H__args
+               (typing_ind Γ T e (C, μ0) H__e)
+               (typing_list_ind Γ T args argsT H__args)
+    | t_call_hot Γ T e m args argTs paramTs D body μ0 μ_r C H__e H__mtd H__args H__hots H__subs =>
+        P_call_hot Γ T e m args argTs paramTs D body μ0 μ_r C H__e H__mtd H__args H__hots H__subs
+                   (typing_ind Γ T e (C, hot) H__e)
+                   (typing_list_ind Γ T args argTs H__args)
+    end
+  with typing_list_ind Γ T el Ul (typing_list: (Γ, T) ⊩ el : Ul) : Pl Γ T el Ul typing_list :=
+         match typing_list with
+         | t_exprs_nil Γ T => Pl_nil Γ T
+         | t_exprs_cons Γ T Ul el U e H__el H__e =>
+             Pl_cons Γ T U Ul e el H__el H__e
+                     (typing_ind Γ T e U H__e)
+                     (typing_list_ind Γ T el Ul H__el)
+         end.
+
+End typing_ind.
