src/OverApproximation.v
@@ -1,0 +1,143 @@
+(* Celsius project *)
+(* Clément Blaudeau - LAMP@EPFL 2021 *)
+(** Store typing *)
+
+From Celsius Require Export MetaTheory Reachability LibTactics.
+Require Import Coq.ssr.ssreflect Coq.ssr.ssrbool Coq.Lists.List Coq.micromega.Psatz Ensembles.
+
+Lemma ot_hot_dom: forall Σ C ω Args Flds Mtds,
+    ct C = class Args Flds Mtds ->
+    Σ ⊨ (C, ω) : (C, hot) ->
+    dom Flds <= dom ω.
+Proof with (meta; eauto with lia).
+  intros.
+  inverts H0.
+  destruct (dom Flds) eqn: H__Flds...
+  lets [ ]: fieldType_exists n H; steps...
+  specialize (H5 n x μ) as [ ]; steps...
+Qed.
+Local Hint Resolve ot_hot_dom: typ.
+
+Lemma ot_warm_dom: forall Σ C ω Args Flds Mtds,
+    ct C = class Args Flds Mtds ->
+    Σ ⊨ (C, ω) : (C, hot) ->
+    dom Flds <= dom ω.
+Proof with (meta; eauto with lia).
+  intros.
+  inverts H0.
+  destruct (dom Flds) eqn: H__Flds...
+  lets [ ]: fieldType_exists n H; steps...
+  specialize (H5 n x μ) as [ ]; steps...
+Qed.
+Local Hint Resolve ot_warm_dom: typ.
+
+
+Lemma object_over_approximation:
+  forall Σ σ (l:Loc) μ,
+    wf σ ->
+    (Σ ⊨ σ) ->
+    (Σ ⊨ l : μ) ->
+    (σ ⊨ l : μ).
+Proof with (meta; eauto with typ rch updates lia).
+  intros ...
+  lets [?C [?ω [?μ ?]]]: H0 H1; steps...
+  destruct (ct C) as [Args Flds Mtds] eqn:H__ct ...
+  destruct μ0 as [ | | Ω | ], μ as [ | | Ω0 |];
+    try solve [invert H5];
+    try apply_anywhere s_mode_cool;
+    try solve [eapply getObj_dom; eauto].
+  - (* hot *)
+    intros l' H__rch.
+    eapply hot_transitivity in H__rch...
+    + lets [?C [?ω [?μ [? [ ]]]]]: H0 H8.
+      destruct (ct C1) as [?Args ?Flds ?Mtds] eqn:?H__ct ...
+      exists C0, ω0, Args0, Flds0, Mtds0; steps...
+    + exists C, (C, hot)...
+  - (* hot ⊑ warm *)
+    exists C ω Args Flds Mtds; steps...
+  - (* hot ⊑ cool Ω *)
+    exists C ω Args Flds Mtds; steps...
+    admit.
+  - (* warm *)
+    exists C ω Args Flds Mtds; steps...
+    eapply wf_proj2 ...
+
+
+
+
+
+
+
+
+        steps.
+
+
+      unfold fieldType; steps... reflexivity.
+      repeat eexists; steps...
+
+    eapply H0 in H6.
+    admit.
+  - (* warm *)
+    + repeat eexists; steps ...
+      apply s_mode_cool in H4.
+      inverts H6 ...
+    + eapply getObj_dom...
+
+  - (* cool *)
+    destruct μ; try solve [invert H4] ...
+    + repeat eexists; steps ...
+      apply s_mode_cool in H4.
+      inverts H6 ...
+    + eapply getObj_dom...
+  - (* cold *)
+    destruct μ; try solve [invert H4] ...
+    eapply getObj_dom...
+Qed.
+
+
+
+
+    inverts H4. admit.
+
+  - (* cold *)
+
+
+  lets : H H0.
+  inverts H1 ; steps.
+  inverts H2 .
+  assert (S l <= dom Σ) by admit.
+  specialize (H l); steps.
+  rewrite H0 in H; invert_constructor_equalities; steps.
+  destruct μ.
+  + assert (μ0 = hot) by (inverts H4; steps); subst.
+    invert H5; steps.
+    intros l' H__l'.
+    destruct (getObj σ l') as [[D ω'] |] eqn:getObj.
+    exists D, ω'. do 3 eexists.
+    split => //.
+    split => //.
+
+  + admit.
+  + admit.
+  + inverts H4.
+
+  inversion H1; steps.
+  inversion H2; steps.
+  specialize (H l); steps.
+  assert (S l <= dom Σ) by admit. steps.
+  inversion H7; steps.
+  + (* hot *)
+    admit.
+  + (* warm *)
+    exists C0, ω.
+  inversion H5; steps.
+
+
+  + (* hot *)
+    admit.
+  + (* warm *)
+    specialize (H l); steps.
+    assert (S l <= dom Σ) by admit. steps.
+    inversion H7; steps.
+    exists C0, ω.
+    inversion H5; steps.
