src/Soundness.v
@@ -1,0 +1,550 @@
+(* Celsius project *)
+(* Clément Blaudeau - Lamp@EPFL 2021 *)
+(** This file defines and proves the soundess of the type system. *)
+
+From Celsius Require Export LocalReasoning Eval.
+Require Import ssreflect ssrbool Psatz Sets.Ensembles List Coq.Sets.Finite_sets_facts Coq.Program.Tactics.
+Import ListNotations Arith.
+Open Scope nat_scope.
+
+Lemma e_this2:
+  forall Γ U T,
+    (Γ, U) ⊢ this : T -> U <: T.
+Proof.
+  intros. remember this as e.
+  induction H; steps; meta; eauto with typ.
+Qed.
+
+Local Hint Constructors evalP: typ.
+Local Hint Constructors T_Expr: typ.
+
+Lemma typ_mtd: forall Γ T__this e m args T,
+    ((Γ, T__this) ⊢ (mtd e m args) : T) ->
+    exists C D e__m argTs paramTs μ__m μ0 μ__r,
+      ((Γ, T__this) ⊢ e : (C, μ0)) /\
+        methodInfo C m = Some (μ__m, paramTs, (D, μ__r),  e__m) /\
+        μ0 ⊑ μ__m /\
+        ((Γ, T__this) ⊩ args : argTs) /\
+        S_Typs argTs paramTs /\
+        ((D, hot) <: T) /\
+        ((D, μ__r) <: T \/ P_hots argTs /\ μ0 = hot).
+Proof with (meta; eauto with typ wf lia).
+  introv H.
+  remember (mtd e m args) as E.
+  induction H; steps...
+  - repeat eexists...
+  - repeat eexists; steps...
+  - repeat eexists...
+    clear IHT_Expr H1 H H0 H2.
+    induction argsT ; eauto using S_Typs with typ...
+  - repeat eexists...
+Qed.
+
+Parameter typable_classes: T_Classes.
+
+Ltac move_top t :=
+  try match goal with
+  | H1:t, H2:t, H3:t, H4:t, H5:t, H6:t, H7:t, H8:t, H9:t |- _ =>
+     move H1 at top;
+     move H2 at top;
+     move H3 at top;
+     move H4 at top;
+     move H5 at top;
+     move H6 at top;
+     move H7 at top;
+     move H8 at top;
+     move H9 at top
+  | H1:t, H2:t, H3:t, H4:t, H5:t, H6:t, H7:t, H8:t |- _ =>
+     move H1 at top;
+     move H2 at top;
+     move H3 at top;
+     move H4 at top;
+     move H5 at top;
+     move H6 at top;
+     move H7 at top;
+     move H8 at top
+  | H1:t, H2:t, H3:t, H4:t, H5:t, H6:t, H7:t |- _ =>
+     move H1 at top;
+     move H2 at top;
+     move H3 at top;
+     move H4 at top;
+     move H5 at top;
+     move H6 at top;
+     move H7 at top
+  | H1:t, H2:t, H3:t, H4:t, H5:t, H6:t |- _ =>
+     move H1 at top;
+     move H2 at top;
+     move H3 at top;
+     move H4 at top;
+     move H5 at top;
+     move H6 at top
+  | H1:t, H2:t, H3:t, H4:t, H5:t |- _ =>
+     move H1 at top;
+     move H2 at top;
+     move H3 at top;
+     move H4 at top;
+     move H5 at top
+  | H1:t, H2:t, H3:t, H4:t |- _ =>
+     move H1 at top;
+     move H2 at top;
+     move H3 at top;
+     move H4 at top
+  | H1:t, H2:t, H3:t |- _ =>
+     move H1 at top;
+     move H2 at top;
+     move H3 at top
+  | H1:t, H2:t |- _ =>
+     move H1 at top;
+     move H2 at top
+  | H1:t |- _ =>
+     move H1 at top
+  end.
+Ltac meta_clean :=
+  move_top StoreTyping;
+  move_top EnvTyping;
+  move_top Env;
+  move_top Store;
+  move_top (list Loc);
+  move_top Loc;
+  move_top (list Tpe);
+  move_top Mode; move_top ClN; move_top Expr.
+
+Ltac modus :=
+  repeat match goal with
+         | H: ?A -> ?B, H': ?A |- _ => specialize (H H')
+         end.
+
+Ltac eval_wf2 :=
+  repeat
+    match goal with
+    | H: codom ?ρ ∪ {?ψ} ⪽ ?σ1, H2: dom ?σ1 <= dom ?σ2 |- _ =>
+        let name := fresh "H__codom" in
+        add_hypothesis name (storeSubset_trans _ σ1 σ2 H2 H)
+    | H:⟦ ?e ⟧p (?σ, ?ρ, ?ψ) --> (?v, ?σ'),
+        H1:wf ?σ,
+          H2 : codom ?ρ ∪ {?ψ} ⪽ ?σ
+      |- _ =>
+        match goal with
+        | H':wf σ' |- _ => fail 1
+        | _ =>
+            let H_val := fresh "H_val" in
+            let H_wf := fresh "H_wf" in
+            pose proof (wf_theorem e σ ρ ψ v σ' H H1 H2) as [H_wf H_val]
+        end
+    | H:⟦_ ?el _⟧p (?σ, ?ρ, ?ψ) --> (?vl, ?σ'),
+        H1:wf ?σ,
+          H2 : codom ?ρ ∪ {?ψ} ⪽ ?σ
+      |- _ =>
+        match goal with
+        | H':wf σ' |- _ => fail 1
+        | _ =>
+            let H_val := fresh "H_val" in
+            let H_wf := fresh "H_wf" in
+            pose proof (wf_theorem_list el σ ρ ψ vl σ' H H2 H1) as [H_wf H_vals]
+        end
+    end.
+
+Definition expr_soundness n e ρ σ ψ r Γ Σ U T :=
+    ((Γ, U) ⊢ e : T) ->
+    (Γ, Σ) ⊨ ρ ->
+    Σ ⊨ σ ->
+    (Σ ⊨ ψ : U) ->
+    wf σ ->
+    (codom ρ ∪ {ψ} ⪽ σ) ->
+    ⟦e⟧(σ, ρ, ψ)(n) = r ->
+    r <> Timeout ->
+    exists Σ' v σ',
+      r = Success v σ' /\
+        Σ ≼ Σ' /\ Σ ≪ Σ' /\ Σ ▷ Σ' /\ (Σ' ⊨ σ') /\ wf σ' /\
+        Σ' ⊨ v : T.
+
+Definition expr_list_soundness n el ρ σ ψ r Γ Σ U Tl :=
+    ((Γ, U) ⊩ el : Tl) ->
+    (Γ, Σ) ⊨ ρ ->
+    Σ ⊨ σ ->
+    (Σ ⊨ ψ : U) ->
+    wf σ ->
+    (codom ρ ∪ {ψ} ⪽ σ) ->
+    ⟦_ el _⟧(σ, ρ, ψ)(n) = r ->
+    r <> Timeout_l ->
+    exists Σ' vl σ',
+      r = Success_l vl σ' /\
+        Σ ≼ Σ' /\ Σ ≪ Σ' /\ Σ ▷ Σ' /\ (Σ' ⊨ σ') /\ wf σ' /\
+        (Tl, Σ') ⊨ vl.
+
+
+Theorem soundness:
+  forall n,
+    (forall e ρ σ ψ r Γ Σ U T,
+        expr_soundness n e ρ σ ψ r Γ Σ U T) /\
+    (forall el ρ σ ψ r Γ Σ U Tl,
+      expr_list_soundness n el ρ σ ψ r Γ Σ U Tl).
+Proof with (
+    meta;
+    meta_clean;
+    eauto 4 with typ wf lia;
+    try match goal with
+        | |- ?Σ ⊨ ?l : ?T => try solve [eapply vt_sub; eauto with typ]
+        end
+  ).
+  induction n as [n IHn] using lt_wf_ind. destruct n;
+    intros; unfold expr_soundness, expr_list_soundness; split; intros;
+    [steps | steps | destruct e | destruct el]; subst;
+    simpl in *...
+  - (* e = var x *)
+    eapply env_regularity in H as (?l & ?H__get & ?)...
+    rewrite H__get in H6 |- * ...
+    exists Σ, l, σ; steps...
+  - (* e = this *)
+    eapply e_this2 in H.
+    exists Σ, ψ, σ; steps...
+  - (* e = fld *)
+    admit.
+  - (* e = mtd e m l *)
+    rename l into args.
+    specialize (IHn n ltac:(lia)) as [IH__expr IH__list]...
+
+    (* Induction on the typing judgment *)
+    eapply typ_mtd in H as
+        (?C & ?C & ?e__m & ?Args & ?Flds & ?μ__m & ?μ' & ?μ__r &
+           HT__e0 & H__mtdinfo & ? & HT__args & HS__args & H__sub & H__hots) ...
+
+    (* Destruct evaluation of e0 *)
+    destruct_eval H__eval0 v σ';
+      lets (Σ0 & v0 & σ0 & H__r & H__mn0 & H__stk0 & H__aty0 & H__st0 & H__wf0 & H__v0) :
+      IH__expr HT__e0 H0 H1 H3 H__eval0; try inverts H__r ...
+    eapply eval_implies_evalp in H__eval0.
+    lets H__pM0: pM_theorem H__eval0.
+    lets (?C & ?ω & ?μ & H__obj & ? & ?): H__st0 H11...
+    rewrite H__obj in H6 |- *.
+
+    (* Destruct method fetch*)
+    unfold methodInfo in H__mtdinfo.
+    destruct (ct C1) as [Args1 Flds1 Mtds1] eqn:H__ct1.
+    destruct (Mtds1 m) as [[?μ__r Ts retT ?] |] eqn:H__Mtds1; [| steps] . inverts H__mtdinfo...
+
+    (* Extract typing for method body from Ξ (well-typed) *)
+    pose proof (typable_classes C1) as HT__em.
+    rewrite H__ct1 in HT__em.
+    destruct HT__em as [_ HT__em].
+    specialize (HT__em m _ _ _ _ H__Mtds1).
+
+    (* Destruct argument evaluation *)
+    lets H__env0: env_typing_monotonicity H__mn0 H0.
+    eval_dom. eval_wf2...
+    lets (?T & ?T & ? & ? & ?): H__mn0 ψ H2...
+    destruct_eval H__eval1 vl σ';
+      lets (Σ1 & args_val & σ1 & H__r & H__mn1 & H__stk1 & H__aty1 & H__st1 & H__wf1 & H__v1) :
+      IH__list HT__args H__env0 H__st0 H__wf0 H__eval1; try inverts H__r ...
+    eapply eval_list_implies_evalp in H__eval1. eval_dom; eval_wf2.
+
+    (* Destruct evaluation of method body *)
+    lets (?T & ?T & ? & ? & ?): H__mn1 ψ H5...
+    lets (?T & ?T & ? & ? & ?): H__mn1 v0 H11...
+    assert (HT__em': (Args, (C1, μ__m)) ⊢ e__m : (C, μ__r)) by admit.
+    destruct (⟦ e__m ⟧ (σ1, args_val, v0 )( n)) as [ | | σ' v' ] eqn:H__eval2; try congruence;
+    lets (Σ2 & v2 & σ2 & H__r & H__mn2 & H__stk2 & H__aty2 & H__st2 & H__wf2 & H__v2) :
+      IH__expr HT__em' H__v1 H__st1 H__wf1 H__eval2; try inverts H__r ... admit. admit.
+    eapply eval_implies_evalp in H__eval2.
+
+    (* Result *)
+    destruct H__hots as [? | [ H__hots ?] ]...
+    + exists Σ2, v2, σ2; repeat split...
+    + (* Local reasoning *)
+      subst...
+      destruct (local_reasoning2 Σ1 Σ2 σ1 σ2 (codom args_val ∪ { v0 }) {v2} ) as
+        (Σ3 & ? & ? & ? & ? & H__v2)...
+      * admit.
+      * admit.
+      * intros ? [l H__l | ? ]; rch_set.
+        admit.
+        admit.
+      * intros l Hl; rch_set.
+
+
+
+
+    destruct H__hots as [H__hots | H__hots]...
+
+    steps...
+    exists (C, μ6)...
+    eapply s_typ_mode.
+    eapply s_mode_trans; eauto.
+    eapply s_mode_trans; eauto.
+
+
+
+    destruct_eval.
+    meta.
+    meta_clean.
+    eauto with typ wf lia.
+    try match goal with
+    | |- ?Σ ⊨ ?l : ?T => try solve [eapply vt_sub; eauto with typ]
+    end.
+    + steps.
+    + clear H8.
+      destruct (getObj s v) as [[?C ?ω] |]. admit.
+      destruct (ct C3) as [?Args ?Flds ?Mtds] eqn:H__ct3.
+      destruct (Mtds m) as [[_ _ _ e1] |]. eqn:H__mtd.
+
+      steps.
+      eapply H8.
+      eapply IHn in H5...
+      congruence. admit. admit.  ; try congruence.
+
+
+
+    exosts
+    rewrite_any.
+    repeat destruct_match; try congruence.
+    admit.
+    destruct
+
+
+
+(** by induction on evaluation *)
+Theorem semantic_soundness:
+    forall e ρ σ ψ l σ',
+      ⟦e⟧p(σ, ρ, ψ) --> (l, σ') ->
+      wf σ ->
+      (codom ρ ∪ {ψ} ⪽ σ) ->
+      forall Γ U T Σ,
+        ((Γ, U) ⊢ e : T) ->
+        (Γ, Σ) ⊨ ρ ->
+        Σ ⊨ σ ->
+        (Σ ⊨ ψ : U) ->
+        exists Σ',
+          Σ ≼ Σ' /\ Σ ≪ Σ' /\ Σ ▷ Σ' /\ (Σ' ⊨ σ') /\ wf σ' /\
+            Σ' ⊨ l : T.
+Proof with (meta; meta_clean; eauto with typ wf lia; try solve [eapply vt_sub; eauto with typ]).
+
+  introv H.
+  induction H using evalP_ind2 with
+    (Pl := fun el σ ρ ψ vl σ' _ =>
+               wf σ ->
+               (codom ρ ∪ {ψ} ⪽ σ) ->
+             forall Γ U Tl Σ,
+               ((Γ, U) ⊩ el : Tl) ->
+               (Γ, Σ) ⊨ ρ ->
+               Σ ⊨ σ ->
+               (Σ ⊨ ψ : U) ->
+               exists Σ',
+                 Σ ≼ Σ' /\ Σ ≪ Σ' /\ Σ ▷ Σ' /\ (Σ' ⊨ σ') /\ wf σ' /\ ((Tl, Σ') ⊨ vl))
+    (Pin := fun C fls I _ σ σ' _   => False );
+    intros; eval_dom; eval_wf2; modus...
+  - (* e_var *)
+    pose proof (env_regularity Γ Σ ρ x (C0,μ0) (C, μ) H2) as [?l [ ]]...
+    exists Σ; steps...
+  - (* e_this *)
+    admit.
+  - (* e_fld *)
+    admit.
+    (* + (* t_sub *) *)
+    (* + (* t_selhot *) *)
+    (* + (* t_selwarm *) *)
+    (* + (* t_selcool *) *)
+  - (* e_mtd *)
+    clear H1 H2 H7 H8 H9 H__codom H__codom0 H__codom1 H_wf H_wf0 H H__el H0.
+    rename H10 into H__getType, H6 into H__inDom, H4 into H__eT, H5 into H__sT.
+    eapply typ_mtd in H3 as
+        (?C & ?C & ?e__m & ?Args & ?Flds & ?μ__m & ?μ' & ?μ__r &
+           HT__e0 & H__mtdinfo & ? & HT__args & HS__args & [? | (H__hot & ?) ] )...
+    + (* t_block *)
+      lets (Σ0 & H__mn0 & H__stk0 & H__aty0 & H__st0 & _ & ?) : IHevalP1 HT__e0 H__eT... clear IHevalP1.
+      lets H__eT0 : env_typing_monotonicity H__mn0 H__eT ...
+      lets (?U1 & ?U2 & ? & ? & ?): H__mn0 H__inDom...
+      lets (Σ__args & H__mnargs & H__stkargs & H__atyargs & H__stargs & _ & H__eTargs) : IHevalP2 HT__args H__eT0...
+      assert (C2 = C). {
+        match goal with
+        | H1: getObj ?σ ?v = Some (?C, ?μ),
+          H2: ?Σ ⊨ ?σ,
+            H3: in_dom ?Σ ?v |- _ =>
+          lets (?C & ?ω & ?μ & ? & ? & ?) : H2 v H3 ; meta
+      end... } subst.
+      unfold methodInfo in *.
+      pose proof (typable_classes C) as H__C. steps...
+      specialize (H8 _ _ _ _ _ matched0) ...
+      lets: H17 H23; steps...
+      lets [Σ__m ?]: IHevalP3 H34; steps ... clear IHevalP3.
+      exists Σ__m; steps...
+
+      * lets: H27 H23; steps...
+      *
+    + (* t_block_call *)
+
+    remember (mtd e0 m el) as e.
+    induction H1; steps ...
+    + (* t_sub *)
+
+      admit.
+    + (* t_block *)
+      admit.
+    + (* t_block_call *)
+      admit.
+    lets [Σ' ?] : IHevalP1 H11 H2; steps... clear IHT_Expr.
+    lets : env_typing_monotonicity H15 H3; clear H0.
+    lets [?U1 [?U2 [? [? ?]]]]: H15 H5...
+    specialize (IHT_Expr0 Σ' ρ ψ (C1, μ6) σ1 vl2 σ2 H20 H_wf) as [Σ'' [ ]]; steps...
+
+    pose proof (typable_classes C).
+    admit.
+  - (* t_call_hot *)
+    admit.
+  - (* tl_nil *)
+    exists ([]: list Loc), σ, Σ; steps...
+  - (* tl_cons *)
+    admit.
+Admitted.
+
+Theorem syntactic_soundness: forall Γ U e T,
+    ((Γ, U) ⊢ e : T) ->
+    forall ρ σ ψ l σ' Σ,
+      ⟦e⟧p(σ, ρ, ψ) --> (l, σ') ->
+      wf σ ->
+      (codom ρ ∪ {ψ} ⪽ σ) ->
+      (Γ, Σ) ⊨ ρ ->
+      Σ ⊨ σ ->
+      (Σ ⊨ ψ : U) ->
+      exists Σ',
+        Σ ≼ Σ' /\ Σ ≪ Σ' /\ Σ ▷ Σ' /\ (Σ' ⊨ σ') /\ wf σ' /\
+          Σ' ⊨ l : T.
+Proof with (meta; eauto with typ wf lia; try solve [eexists; eauto with typ]).
+
+  introv H.
+  induction H using typing_ind with
+    (Pl := fun Γ T el Ul _ => forall Σ ρ ψ (U:Tpe) σ vl σ',
+               ⟦_ el _⟧p (σ, ρ, ψ) --> (vl, σ') ->
+               wf σ ->
+               (codom ρ ∪ {ψ} ⪽ σ) ->
+               (Γ, Σ) ⊨ ρ ->
+               Σ ⊨ σ ->
+               (Σ ⊨ ψ : U) ->
+               exists Σ',
+                   Σ ≼ Σ' /\ Σ ≪ Σ' /\ Σ ▷ Σ' /\ (Σ' ⊨ σ') /\ wf σ' /\
+                   (forall l, List.In l vl -> Σ' ⊨ l : T));
+    intros ...
+  - (* t_sub *)
+    lets  [Σ' ?] : IHT_Expr H0 H1; steps... clear IHT_Expr.
+    exists Σ'; steps...
+  - (* t_var *)
+    pose proof (env_regularity Γ Σ ρ x (C0,μ1) (C, μ) H2) as [?l [ ]]...
+    inverts H.
+    exists Σ; steps...
+  - (* t_this *)
+    inverts H.
+    exists Σ; steps...
+  - (* t_selhot *)
+    inverts H0.
+    lets [Σ' ?] : IHT_Expr H10 H3; steps... clear IHT_Expr.
+    lets [?C [?ω [?μ ?]]]: H12 H15; steps...
+    lets [?v [ ]]: hot_selection l1 H13 H12 H19 H__field...
+    exists Σ'; steps...
+  - (* t_selwarm *)
+    inverts H0.
+    lets [Σ' ?] : IHT_Expr H10 H3; steps... clear IHT_Expr.
+    lets [?C [?ω [?μ ?]]]: H12 H15; steps...
+    lets [?v [ ]]: warm_selection l1 H12 H19 H__field...
+    exists Σ'; steps...
+  - (* t_selcool *)
+    inverts H0.
+    lets [Σ' ?] : IHT_Expr H10 H3; steps... clear IHT_Expr.
+    lets [?C [?ω [?μ ?]]]: H12 H15; steps...
+    lets [?v [ ]]: cool_selection l1 Ω H12 H19 H__field...
+    exists Σ'; steps...
+  - (* t_new *)
+    admit.
+  - (* t_new_hot *)
+    admit.
+  - (* t_block *)
+    admit.
+  - (* t_call *)
+    inverts H0. eval_dom; eval_wf.
+    lets [Σ' ?] : IHT_Expr H11 H2; steps... clear IHT_Expr.
+    lets : env_typing_monotonicity H15 H3; clear H0.
+    lets [?U1 [?U2 [? [? ?]]]]: H15 H5...
+    specialize (IHT_Expr0 Σ' ρ ψ (C1, μ6) σ1 vl2 σ2 H20 H_wf) as [Σ'' [ ]]; steps...
+
+    pose proof (typable_classes C).
+    admit.
+  - (* t_call_hot *)
+    admit.
+  - (* tl_nil *)
+    exists ([]: list Loc), σ, Σ; steps...
+  - (* tl_cons *)
+    admit.
+Admitted.
+
+Parameter typable_classes : T_Classes.
+
+Theorem expression_soundness: forall e Γ Σ σ U T ρ ψ,
+    ((Γ, U) ⊢ e : T) ->
+    (Γ, Σ) ⊨ ρ ->
+    Σ ⊨ σ ->
+    (Σ ⊨ ψ : U) ->
+    wf σ ->
+    exists l σ' Σ',
+      ⟦e⟧(σ, ρ, ψ) --> (l, σ') /\
+        Σ ≼ Σ' /\ Σ ≪ Σ' /\ Σ ▷ Σ' /\ (Σ' ⊨ σ') /\ wf σ' /\
+        Σ' ⊨ l : T.
+Proof with (meta; eauto with typ; try solve [eexists; eauto with typ]).
+  intros. gen Σ ρ ψ σ.
+  induction H using typing_ind with
+    (Pl := fun Γ T el Ul _ => forall Σ ρ ψ U σ,
+               (Γ, Σ) ⊨ ρ ->
+               Σ ⊨ σ ->
+               (Σ ⊨ ψ : U) ->
+               wf σ ->
+               exists vl σ' Σ',
+                 ⟦_ el _⟧p (σ, ρ, ψ) --> (vl, σ') /\
+                   Σ ≼ Σ' /\ Σ ≪ Σ' /\ Σ ▷ Σ' /\ (Σ' ⊨ σ') /\ wf σ' /\
+                   (forall l, List.In l vl -> Σ' ⊨ l : T));
+    intros ...
+  - (* t_sub *)
+    lets  [l [σ' [Σ' ?]]] : IHT_Expr H0 ψ H1; steps... clear IHT_Expr.
+    exists l, σ', Σ'; steps...
+  - (* t_var *)
+    pose proof (env_regularity Γ Σ ρ x (C0,μ1) (C, μ) H0) as [?l [ ]]...
+    exists l, σ, Σ; steps...
+    apply e_var...
+  - (* t_this *)
+    exists ψ, σ, Σ; steps...
+  - (* t_selhot *)
+    lets [l [σ' [Σ' ?]]] : IHT_Expr H0 ψ H1; steps... clear IHT_Expr.
+    lets [?C [?ω [?μ ?]]]: H10 H13; steps...
+    lets [?v [ ]]: hot_selection l H11 H10 H15 H__field...
+    exists v σ' Σ'; steps...
+    eapply e_fld...
+  - (* t_selwarm *)
+    lets [l [σ' [Σ' ?]]] : IHT_Expr H0 ψ H1; steps... clear IHT_Expr.
+    lets [?C [?ω [?μ ?]]]: H10 H13; steps...
+    lets [?v [ ]]: warm_selection l H10 H15 H__field...
+    exists v σ' Σ'; steps...
+    eapply e_fld...
+  - (* t_selcool *)
+    lets [l [σ' [Σ' ?]]] : IHT_Expr H0 ψ H1; steps... clear IHT_Expr.
+    lets [?C [?ω [?μ ?]]]: H10 H13; steps...
+    lets [?v [ ]]: cool_selection l Ω H10 H15 H__field...
+    exists v σ' Σ'; steps...
+    eapply e_fld...
+  - (* t_new *)
+    admit.
+  - (* t_new_hot *)
+    admit.
+  - (* t_block *)
+    admit.
+  - (* t_call *)
+    lets [l [σ' [Σ' ?]]] : IHT_Expr H0 ψ H1; steps... clear IHT_Expr.
+    lets [U1 [U2 [? [ ]]]]: H5 ψ H2 ...
+    clear H1 H3 H6 H2 H14.
+    lets : env_typing_monotonicity H5 H0; clear H0.
+    lets [?C [?ω [?μ ?]]]: H10 H13; steps...
+    specialize (IHT_Expr0 Σ' ρ ψ C1 σ' H1 H10) as [vl [σ'' [Σ'' [ ]]]]; steps... exists μ4 ...
+    pose proof (typable_classes C).
+    admit.
+  - (* t_call_hot *)
+    admit.
+  - (* tl_nil *)
+    exists ([]: list Loc), σ, Σ; steps...
+  - (* tl_cons *)
+    admit.
+Admitted.
